day02_1, proof progress

day02_1.v
@@ -19,20 +19,29 @@ Module Algorithm (Import OT : OrderedType.OrderedType).
 
 Module Map := FMapAVL.Make OT.
 
-Fixpoint collect_aux (xs : list t) (count : Map.t nat) :
-  Map.t nat :=
-  match xs with
-  | [] => count
-  | x :: xs =>
+(* Interpret a finite map [Map.t nat] as a function [t -> nat],
+   defaulting to 0 outside of its support. *)
+Definition lookup (count : Map.t nat) : t -> nat :=
+  fun x : t =>
     match Map.find x count with
-    | None => collect_aux xs (Map.add x 1 count)
-    | Some n => collect_aux xs (Map.add x (1+n) count)
-    end
-  end.
+    | None => 0
+    | Some n => n
+    end.
 
+(* Increment the value associated to [x] by one. *)
+Definition increment (x : t) : Map.t nat -> Map.t nat :=
+  fun count => Map.add x (1 + lookup count x) count.
+
+(* [collect xs] gives, for every element [x : t], the number
+   of times it occues in [xs]. *)
 Definition collect (xs : list t) : Map.t nat :=
-  collect_aux xs (Map.empty nat).
+  fold_left
+    (fun count x => increment x count)
+    xs
+    (Map.empty nat).
 
+(* Now it is straightforward to determine whether some element
+   occurs two or three times in the list [xs]. *)
 Definition two_or_three (xs : list t) : bool * bool :=
   Map.fold (fun _ n tot =>
               (fst tot || (n =? 2), snd tot || (n =? 3))%bool)
@@ -48,6 +57,9 @@ Section main.
 Context {m : Type -> Type} `{Monad m}
         `{MonadI (list ascii) m} `{MonadO nat m} `{MonadFix m}.
 
+(* We have two counters for the numbers of words containing
+   two/three of any letter. For each word, [two_or_three] tells us
+   whether to increment each counter. *)
 Definition main : m unit :=
   mfix (fun loop '(twos, threes) =>
     oid <- read;;
@@ -67,3 +79,182 @@ Import SimpleIO.
 Definition exec : io_unit := IO.unsafe_run main.
 
 Extraction "day02_1.ml" exec.
+
+Section spec.
+
+(* We first formalize the property of having exactly two/three
+   of a given letter. *)
+
+(* The number of occurences of [c] in [xs]. *)
+Definition n_occurs (c : ascii) (xs : list ascii) : nat :=
+  List.length (filter (eqb_ascii c) xs).
+
+(* [has_n n xs : Prop] holds when some letter appears in [xs]
+   exactly [n] times. *)
+Definition has_n (n : nat) (xs : list ascii) : Prop :=
+  exists c, n_occurs c xs = n.
+
+Definition has_two : list ascii -> Prop := has_n 2.
+Definition has_three : list ascii -> Prop := has_n 3.
+
+(* The meat of the program: [two_or_three].
+
+   We first state the specification of [two_or_three], and then prove
+   properties about the surrounding auxiliary functions until
+   we can prove that spec. *)
+
+(* The two booleans of [two_or_three] tell us whether there are
+   elements occuring two/three times in the list [xs]. *)
+Definition two_or_three_spec : Prop :=
+  forall xs : list ascii,
+    (fst (two_or_three xs) = true <-> has_two xs) /\
+    (snd (two_or_three xs) = true <-> has_three xs).
+
+Lemma increment_plus_one x count :
+  lookup (increment x count) x = S (lookup count x).
+Proof.
+  unfold increment, lookup.
+  destruct (Map.find x count) as [n |] eqn:e_find.
+  - apply Map.find_2 in e_find.
+    erewrite Map.find_1; [eauto |].
+    apply Map.add_1; auto.
+  - erewrite Map.find_1; [eauto |].
+    apply Map.add_1; auto.
+Qed.
+
+Lemma Map_find_None {A : Type} y (m : Map.t A) :
+  (forall e, ~ Map.MapsTo y e m) <-> Map.find y m = None.
+Proof.
+  split.
+  - intros H. destruct Map.find as [a | ] eqn:e_find; auto.
+    apply Map.find_2 in e_find. firstorder.
+  - intros H e HM. apply Map.find_1 in HM.
+    rewrite HM in H. discriminate.
+Qed.
+
+Lemma Map_add_neq {A : Type} (m : Map.t A) (x y : Map.key) (e e' : A) :
+  x <> y -> (Map.MapsTo y e (Map.add x e' m) <-> Map.MapsTo y e m).
+Proof.
+  split. { apply Map.add_3; auto. } { apply Map.add_2; auto. }
+Qed.
+
+Lemma Map_find_add_neq  {A : Type} (m : Map.t A) x y e :
+  x <> y -> Map.find y (Map.add x e m) = Map.find y m.
+Proof.
+  intros Hneq.
+  destruct (Map.find y m) as [e' |] eqn:e_find.
+  - apply Map.find_1, Map.add_2, Map.find_2; auto.
+  - apply Map_find_None.
+    intros e' HM.
+    apply Map.add_3 in HM; auto.
+    apply Map.find_1 in HM.
+    rewrite HM in e_find. discriminate.
+Qed.
+
+Lemma increment_id x y count :
+  x <> y -> lookup (increment x count) y = lookup count y.
+Proof.
+  intro Hneq.
+  unfold increment, lookup.
+  destruct (Map.find y count) as [n |] eqn:e_find.
+  - erewrite Map.find_1; [eauto |].
+    apply Map.add_2; auto.
+    apply Map.find_2; auto.
+  - rewrite Map_find_add_neq; auto.
+    rewrite e_find; auto.
+Qed.
+
+(* A translation and proof of the specification of [collect]
+   stated earlier. *)
+Lemma collect_correct :
+  forall xs c, lookup (collect xs) c = n_occurs c xs.
+Proof.
+  unfold collect.
+  assert (H : forall xs c (count : Map.t nat),
+             lookup (fold_left
+               (fun count x => increment x count)
+               xs
+               count) c = n_occurs c xs + lookup count c).
+  { induction xs as [| x xs]; simpl; auto.
+    intros c count.
+    unfold n_occurs. simpl.
+    destruct eqb_ascii eqn:e_cx.
+    - apply eqb_eq in e_cx; subst.
+      simpl.
+      rewrite <- Nat.add_succ_r.
+      rewrite <- increment_plus_one.
+      apply IHxs.
+    - rewrite neqb_neq in e_cx.
+      erewrite <- (increment_id _ _ count); eauto.
+  }
+  intros.
+  specialize (H xs c (Map.empty nat)); unfold lookup in H; simpl in H.
+  rewrite plus_0_r in H.
+  auto.
+Qed.
+
+Lemma fold_left_ind {A B : Type} (P : list A -> B -> B -> Prop)
+      (f : B -> A -> B)
+      (Hnil : forall y, P [] y y)
+      (Hcons : forall x xs y y', P xs (f y x) y' -> P (x :: xs) y y') :
+  forall xs y,
+    P xs y (fold_left f xs y).
+Proof.
+  induction xs as [| x xs]; auto.
+  simpl; firstorder.
+Qed.
+
+Theorem two_or_three_correct : two_or_three_spec.
+Proof.
+  intro xs.
+  remember (two_or_three xs) as ttx eqn:ettx.
+  unfold two_or_three in ettx.
+  rewrite Map.fold_1 in ettx.
+  match type of ettx with
+  | (_ = fold_left ?f _ _) =>
+    assert (H : forall xs y,
+               (fst (fold_left f xs y) = true <->
+                (exists c, List.In (c, 2) xs) \/ fst y = true))
+  end.
+  { clear.
+    induction xs; intros [t1 t2].
+    - firstorder.
+    - simpl. split.
+      + intro H0.
+        apply IHxs in H0. simpl in H0.
+        destruct H0 as [[c H0] | H0].
+        * firstorder.
+        * apply Bool.orb_prop in H0.
+          destruct H0; auto.
+          rewrite Nat.eqb_eq in H.
+          destruct a as [c p]; left; exists c. auto.
+      + intros H0. apply IHxs.
+        destruct H0 as [[c [H | H]]| H].
+        * subst a; auto. simpl. rewrite Bool.orb_true_r; auto.
+        * left. exists c; auto.
+        * subst; auto.
+  }
+  split.
+  - subst ttx. rewrite H.
+    split.
+    + intros [[c Hc]|]; [| discriminate].
+      exists c.
+      rewrite <- collect_correct.
+      unfold lookup.
+      erewrite Map.find_1; auto.
+      apply Map.elements_2, SetoidList.In_InA; auto.
+      typeclasses eauto.
+    + intros [c Hc]. left.
+      rewrite <- collect_correct in Hc.
+      unfold lookup in Hc.
+      destruct Map.find eqn:ec in Hc; [| discriminate].
+      exists c.
+      apply Map.find_2 in ec.
+      apply Map.elements_1 in ec.
+      apply SetoidList.InA_alt in ec.
+      destruct ec as [[c' n'] []].
+      inversion H0; simpl in *; subst; auto.
+  - admit.
+Abort.
+
+End spec.
